#### Example 1

[Ground-truth Solution]:
First, we move all terms to one side to get $4x^2 - 3x + 12 = 0.$ Seeing that factoring will not work, we apply the Quadratic Formula: \begin{align*}
x &= \frac{-(-3) \pm \sqrt{(-3)^2 - 4(4)(12)}}{2 (4)}\\
&= \frac{3 \pm \sqrt{9 - 192}}{8} = \frac{3 \pm \sqrt{-183}}{8} = \frac{3}{8} \pm \frac{\sqrt{183}}{8}i.
\end{align*}Now we see that $a = \dfrac{3}{8}$ and $b = \pm \frac{\sqrt{183}}{8},$ so $a + b^2 = \dfrac{3}{8} + \dfrac{183}{64} = \boxed{\dfrac{207}{64}}.$

[Error-Injected Solution]:
Let's think step by step
We rewrite the equation as $4x^2 - 3x + 12 = 0$,
then apply the quadratic formula to get
\[x = \frac{3 \pm \sqrt{(-3)^2 - 4 \cdot 4 \cdot 12}}{2 \cdot 4} = \frac{3 \pm \sqrt{-183}}{8} = \frac{3}{8} \pm \frac{\sqrt{183}}{8} i,\]so $a = \frac{3}{8}$ and $b = \frac{\sqrt{183}}{8},$ and $a + b^2 = \frac{3}{8} + \left(\frac{\sqrt{183}}{8}\right)^2 = \frac{3}{8} + \frac{183}{64} = \frac{18 + 183}{64} = \boxed{\frac{201}{64}}$.
The answer is: \frac{201}{64}

<explanation>
The error in this solution is a 'calculation_error'. The first wrong step arises because the proposed solution incorrectly calculates the value of \( a + b^2 \). The correct value should be \( \frac{3}{8} + \frac{183}{64} \), but the proposed solution simplifies this to \( \frac{18 + 183}{64} \), which is incorrect. The correct simplification should be \( \frac{24 + 183}{64} = \frac{207}{64} \).
</explanation>

#### Example 2

[Question]:
Let $\mathbf{M} = \begin{pmatrix} 2 & 7 \\ -3 & -1 \end{pmatrix}.$  There exist scalars $p$ and $q$ such that
\[\mathbf{M}^2 = p \mathbf{M} + q \mathbf{I}.\]Enter the ordered pair $(p,q).$

[Ground-truth Solution]:
Since $\mathbf{M}^2 = \begin{pmatrix} 2 & 7 \\ -3 & -1 \end{pmatrix} \begin{pmatrix} 2 & 7 \\ -3 & -1 \end{pmatrix} = \begin{pmatrix} -17 & 7 \\ -3 & -20 \end{pmatrix},$ we seek $p$ and $q$ such that
\[\begin{pmatrix} -17 & 7 \\ -3 & -20 \end{pmatrix} = p \begin{pmatrix} 2 & 7 \\ -3 & -1 \end{pmatrix} + q \begin{pmatrix} 1 & 0 \\ 0 & 1 \end{pmatrix}.\]Thus, we want $p$ and $q$ to satisfy $2p + q = -17,$ $7p = 7,$ $-3p = -3,$ and $-p + q = -20.$  Solving, we find $(p,q) = \boxed{(1,-19)}.$

[Error-Injected Solution]:
Let's think step by step
We have $\mathbf{M}^2 =\begin{pmatrix} 2 & 7 \\ -3 & -1 \end{pmatrix} \begin{pmatrix} 2 & 7 \\ -3 & -1 \end{pmatrix} = \begin{pmatrix} -17 & 7 \\ -9 & -10 \end{pmatrix}.$
We can factor out a $-1$ on the right to get $\mathbf{M}^2 = -1 \begin{pmatrix} 17 & -7 \\ 9 & 10 \end{pmatrix}.$
Setting this equal to $p \mathbf{M} + q \mathbf{I},$ we get $\begin{pmatrix} -17 & 7 \\ -9 & -10 \end{pmatrix} = p\begin{pmatrix} 2 & 7 \\ -3 & -1 \end{pmatrix} + q\begin{pmatrix} 1 & 0 \\ 0 & 1 \end{pmatrix}.$
This gives the system of equations
\begin{align*}
2p + q &= -17, \\
7p &= 7,
\end{align*}which has solution $(p,q) = \boxed{(-10,-3)}.$
The answer is: (-10,-3)
<explanation>
I inject a 'calculation_error' into the solution. The first wrong step arises because the matrix $\mathbf{M}^2$ was calculated incorrectly. The correct calculation should be $\mathbf{M}^2 = \begin{pmatrix} -17 & 7 \\ -3 & -20 \end{pmatrix}$, but the proposed solution incorrectly computes it as $\begin{pmatrix} -17 & 7 \\ -9 & -10 \end{pmatrix}$. 
</explanation>