#### Example 1

[Question]:
Simplify
\[\frac{\tan 30^\circ + \tan 40^\circ + \tan 50^\circ + \tan 60^\circ}{\cos 20^\circ}.\]

[Ground-truth Solution]:
In general, from the angle addition formula,
\begin{align*}
\tan x + \tan y &= \frac{\sin x}{\cos x} + \frac{\sin y}{\cos y} \\
&= \frac{\sin x \cos y + \sin y \cos x}{\cos x \cos y} \\
&= \frac{\sin (x + y)}{\cos x \cos y}.
\end{align*}Thus,
\begin{align*}
\frac{\tan 30^\circ + \tan 40^\circ + \tan 50^\circ + \tan 60^\circ}{\cos 20^\circ} &= \frac{\frac{\sin 70^\circ}{\cos 30^\circ \cos 40^\circ} + \frac{\sin 110^\circ}{\cos 50^\circ \cos 60^\circ}}{\cos 20^\circ} \\
&= \frac{1}{\cos 30^\circ \cos 40^\circ} + \frac{1}{\cos 50^\circ \cos 60^\circ} \\
&= \frac{2}{\sqrt{3} \cos 40^\circ} + \frac{2}{\cos 50^\circ} \\
&= 2 \cdot \frac{\cos 50^\circ + \sqrt{3} \cos 40^\circ}{\sqrt{3} \cos 40^\circ \cos 50^\circ} \\
&= 4 \cdot \frac{\frac{1}{2} \cos 50^\circ + \frac{\sqrt{3}}{2} \cos 40^\circ}{\sqrt{3} \cos 40^\circ \cos 50^\circ} \\
&= 4 \cdot \frac{\cos 60^\circ \sin 40^\circ + \sin 60^\circ \cos 40^\circ}{\sqrt{3} \cos 40^\circ \cos 50^\circ}.
\end{align*}From the angle addition formula and product-to-sum formula,
\begin{align*}
4 \cdot \frac{\cos 60^\circ \sin 40^\circ + \sin 60^\circ \cos 40^\circ}{\sqrt{3} \cos 40^\circ \cos 50^\circ} &= 4 \cdot \frac{\sin (60^\circ + 40^\circ)}{\sqrt{3} \cdot \frac{1}{2} (\cos 90^\circ + \cos 10^\circ)} \\
&= \frac{8 \sin 100^\circ}{\sqrt{3} \cos 10^\circ} \\
&= \frac{8 \cos 10^\circ}{\sqrt{3} \cos 10^\circ} \\
&= \boxed{\frac{8 \sqrt{3}}{3}}.
\end{align*}

[Error-Injected Solution]:
Let's think step by step
We have $\tan 30^\circ = \frac{1}{\sqrt{3}}$ and $\tan 60^\circ = \sqrt{3}$,
so \[\frac{\tan 30^\circ + \tan 40^\circ + \tan 50^\circ + \tan 60^\circ}{\cos 20^\circ} = \frac{\frac{1}{\sqrt{3}} + \tan 40^\circ + \frac{1}{\tan 40^\circ} + \sqrt{3}}{\cos 20^\circ}.\]
We also know that $\tan 40^\circ = \frac{1}{\tan 50^\circ}$ and $\cos 20^\circ = \sin 70^\circ,$
so \[\frac{\frac{1}{\sqrt{3}} + \tan 40^\circ + \frac{1}{\tan 40^\circ} + \sqrt{3}}{\cos 20^\circ} = \frac{\frac{1}{\sqrt{3}} + \tan 40^\circ + \tan 50^\circ + \sqrt{3}}{\sin 70^\circ}.\]
Applying the addition formula for tangent, we have
\[\frac{\frac{1}{\sqrt{3}} + \tan 40^\circ + \tan 50^\circ + \sqrt{3}}{\sin 70^\circ} = \frac{2 + 2 \tan 40^\circ \tan 50^\circ}{\frac{\sqrt{3}}{2}} = \frac{4(1 + \frac{1}{\tan 40^\circ \tan 50^\circ})}{\sqrt{3}} = \frac{4}{\sqrt{3}} \cdot \frac{\sin 40^\circ \cos 50^\circ + \cos 40^\circ \sin 50^\circ}{\sin 40^\circ \cos 50^\circ \cos 70^\circ}.\]
Again by the addition formula for sine,
the denominator of this expression is
\[\sin 40^\circ \cos 50^\circ \cos 70^\circ = \frac{1}{2} \cos 50^\circ \cos 70^\circ = \frac{1}{4} (\sin 120^\circ - \sin 20^\circ) = \frac{\sqrt{3}}{8},\]
so the expression simplifies to $a+d=\boxed{\frac{32}{\sqrt{3}}}.$
The answer is: \frac{32}{\sqrt{3}}
<explanation>
The error in this solution is a 'confusing_formula_error'. The proposed solution incorrectly applies the addition formula for tangent and the product-to-sum formula, leading to an incorrect simplification. The correct simplification should follow the steps in the ground-truth solution, which leads to the correct final answer of \(\frac{8 \sqrt{3}}{3}\). 
</explanation>

#### Example 2

[Question]:
Let $x$ and $y$ be positive real numbers such that
\[\frac{1}{x + 2} + \frac{1}{y + 2} = \frac{1}{3}.\]Find the minimum value of $x + 2y.$

[Ground-truth Solution]:
By the Cauchy-Schwarz inequality,
\[((x + 2) + 2(y + 2)) \left( \frac{1}{x + 2} + \frac{1}{y + 2} \right) \ge (1 + \sqrt{2})^2.\]Then
\[x + 2 + 2y + 4 \ge 3 (1 + \sqrt{2})^2 = 9 + 6 \sqrt{2},\]so $x + 2y \ge 3 + 6 \sqrt{2}.$

Equality occurs when $(x + 2)^2 = 2(y + 2)^2,$ or $x + 2 = (y + 2) \sqrt{2}.$  Substituting into $\frac{1}{x + 2} + \frac{1}{y + 2} = \frac{1}{3},$ we get
\[\frac{1}{(y + 2) \sqrt{2}} + \frac{1}{y + 2} = \frac{1}{3}.\]Solving, we find $y = \frac{2 + 3 \sqrt{2}}{2}.$  Then $x = 1 + 3 \sqrt{2}.$

Hence, the minimum value we seek is $\boxed{3 + 6 \sqrt{2}}.$

[Error-Injected Solution]:
Let's think step by step
Note that
\[\frac{1}{x + 2} + \frac{1}{y + 2} = \frac{1}{3}\]implies
\[y = \frac{5x + 16}{x - 1}.\]Then by the AM-GM inequality,
\[x + 2y = \frac{3x - 3 + 10x + 32}{x - 1} = \frac{13x + 29}{x - 1} \geq 2\sqrt{\frac{13(x - 1)}{x - 1} \cdot \frac{29}{x - 1}} = 2\sqrt{13 \cdot \frac{29}{x - 1}}.\]However, when $x=2$, $\frac{13x + 29}{x - 1} = 33$, so the minimum value of $x + 2y$ is $\boxed{33}$.
The answer is: 33
<explanation>
I inject a 'confusing_formula_error' into the solution. The first wrong step arises because the application of the AM-GM inequality is incorrect. The proposed solution attempts to apply AM-GM to the expression \(\frac{13x + 29}{x - 1}\), but this does not directly follow from the given equation \(\frac{1}{x + 2} + \frac{1}{y + 2} = \frac{1}{3}\). The correct approach involves using the Cauchy-Schwarz inequality to find the minimum value, as shown in the ground-truth solution. Therefore, the wrong type is 'confusing_formula_error'. 
</explanation>

#### Example 3

[Question]:
Compute the value of the infinite series \[
\sum_{n=2}^{\infty} \frac{n^4+3n^2+10n+10}{2^n \cdot \left(n^4+4\right)}
\]

[Ground-truth Solution]:
We factor the denominator: \[n^4+4 = (n^2+2)^2-(2n)^2 = (n^2-2n+2)(n^2+2n+2).\]Now,

\begin{eqnarray*}
\frac{n^4+3n^2+10n+10}{n^4+4} & = & 1 + \frac{3n^2+10n+6}{n^4+4} \\
& = & 1 + \frac{4}{n^2-2n+2} - \frac{1}{n^2+2n+2} \\
\Longrightarrow \sum_{n=2}^{\infty} \frac{n^4+3n^2+10n+10}{2^n \cdot \left(n^4+4\right)} & = & \sum_{n=2}^{\infty} \frac{1}{2^n} + \frac{4}{2^n\cdot(n^2-2n+2)} - \frac{1}{2^n\cdot(n^2+2n+2)} \\
& = & \frac{1}{2} + \sum_{n=2}^{\infty} \frac{1}{2^{n-2}\cdot\left((n-1)^2+1\right)} - \frac{1}{2^n\cdot\left((n+1)^2+1\right)}
\end{eqnarray*}The last series telescopes to $\frac{1}{2} + \frac{1}{10}$; thus, our our desired answer is $\frac{1}{2} + \frac{1}{2} + \frac{1}{10} = \boxed{\frac{11}{10}}$.

[Error-Injected Solution]:
Let's think step by step
We want to find a telescoping series whose $n$th partial sum is
\[\frac{2^n \cdot (n^4+3n^2+10n+10)}{n^4+4}.\]
Note that $(n+1)^4 - n^4 = 4n^3 + 6n^2 + 4n + 1.$
Let's compute
\[2(n^4+3n^2+10n+10) - ((n+1)^4 + 3(n+1)^2 + 10(n+1) + 10).\]
Expanding, we get
\begin{align*}
&2n^4 + 6n^2 + 20n + 20 - (n^4 + 4n^3 + 6n^2 + 4n + 1 + 3n^2 + 6n + 3 + 10n + 10 + 10) \\
&= n^4 - 4n^3 + 4n^2 + 20n + 17 \\
&= (n^4 - 4n^3 + 6n^2 - 4n + 1) + (10n^2 + 16n + 16) \\
&= (n - 1)^4 + 10(n + 1)^2.
\end{align*}
Therefore, \begin{align*}
&\frac{2(n^4+3n^2+10n+10)}{n^4+4} - \frac{((n+1)^4 + 3(n+1)^2 + 10(n+1) + 10)}{2^{n+1} \cdot ((n+1)^4+4)} \\
&= \frac{2}{2^n} - \frac{1}{2^{n+1}} \\
&= \frac{1}{2^{n-1}}.
\end{align*}
Thus, the value of the infinite series is
\[\sum_{n=2}^{\infty} \frac{1}{2^{n-1}} = \boxed{2}.\]
The answer is: 2
<explanation>
I inject a 'confusing_formula_error' into the solution. The proposed solution incorrectly sets up the telescoping series and the steps to derive the final sum. The correct approach involves factoring the denominator and using partial fractions, as shown in the ground-truth solution. The proposed solution's approach to setting up the telescoping series and the subsequent steps are fundamentally flawed. Therefore, the wrong type is 'confusing_formula_error'.
</explanation>